\begin{frame}{SAT motivation}
  \begin{description}
    \item[SAT] is short for Boolean SATisfiability.
    \item[It is] the archetypal NP-complete problem.
    \item[Informally] it asks if there is a way to efficiently decide if an expression containing a bunch of Boolean variables combined using ands, ors, nots and brackets has any setting of the variables that makes the expression true.
  \end{description}

  \begin{exampleblock}{SAT instance example}
    Consider the expression $(x_1 \lor \neg{x_2}) \land (\neg{x_1} \lor x_2 \lor x_3) \land \neg{x_1}$, where $x_1$, $x_2$ and $x_3$ are true/false variables.
    Is there any setting of the variables that makes the expression true?
  \end{exampleblock}
\end{frame}


\begin{frame}{Propositional logic}
  \begin{description}
    \item[Literals] are Boolean variables (can be True or False), and their negations. They are represented by lower case letters like $a$ and $x_i$.
    \vspace{0.3cm}
    \item[Clause] are expressions based on literals, that evaluate as True or False based on the literals. We use not, and and or on the literals. We'll sometimes call them expressions.
    \vspace{0.3cm}
    \item[Not] is depicted by $\neg$. So ``not $a$'' is denoted by $\neg a$.
    \vspace{0.3cm}
    \item[Or] is depicted by $\lor$. So ``$a$ or $b$'' is denoted by $a \lor b$.
    \vspace{0.3cm}
    \item[And] is depicted by $\land$. So ``$a$ and $b$'' is denoted by $a \land b$.
  \end{description}
\end{frame}


\begin{frame}{Normal forms}
  \begin{description}
    \item[CNF] A clause is in Conjunctive Normal Form if it is a ``conjunction of disjunctions'': $(a \lor b) \land (\neg a \lor c) \land d$.
    \vspace{0.5cm}
    \item[DNF] A clause is in Disjunctive Normal Form if it is a ``disjunction of conjunctions'': $(a \land b) \lor (\neg a \land c) \lor d$.
  \end{description}
  
  \vspace{4mm}
  \begin{alertblock}{Converting to CNF and DNF}
    Every Boolean expression can be converted to CNF, and every Boolean expression can also be converted to DNF.
  \end{alertblock}
\end{frame}


\begin{frame}{Four laws}
  The following four laws can be used to convert expressions to CNF and DNF.
  The first two are known as De Morgan's laws, and the latter two are called the distributivity laws.
  \vspace{4mm}
  \begin{alertblock}{Conversion laws}
    \[ \neg ( a \lor b) = \neg a \land \neg b \]
    \[ \neg ( a \land b) = \neg a \lor \neg b \]
    \[ c \land ( a \lor b) = (c \land a) \lor (c \land b) \]
    \[ c \lor ( a \land b) = (c \lor a) \land (c \lor b) \]
  \end{alertblock}
\end{frame}


\begin{frame}{Boolean Satisfiability Problem (SAT)}
  \begin{description}
    \item[SAT] is the set of all Boolean expressions that are satisfiable.
    \item[Satisfiable] expressions have some setting of their constituent variables that causes them to evaluate as true.
    \item[The SAT decision problem] is the problem of deciding which Boolean expressions are in SAT.
    \item[Note] that it's easy to verify that a given setting of the variables in an expression make it true.
  \end{description}
\end{frame}


\begin{frame}{$k$-SAT}
  $k$-SAT is like SAT except that all expressions must be in CNF and each clause must be a disjunction of $k$ literals.

  \vspace{2mm}

  \begin{description}
    \item[2-SAT] example: $(a \lor b) \land (\neg c \lor d) \land \ldots$
    \item[2-SAT] is not NP-complete. There are polynomial time algorithms that solve it.
    \item[3-SAT] example: $(a \lor b \lor c) \land (\neg c \lor d \lor \neg a) \land \ldots$
    \item[3-SAT] is NP complete.
  \end{description}
\end{frame}


\begin{frame}{3-SAT is NP-Complete}

  \begin{alertblock}{Reduction}
    3-SAT is a special case of SAT, so 3-SAT must be in NP.
    We can reduce SAT to 3-SAT in polynomial time.
    First take the expression and convert it to a CNF expression (in polynomial time).
    Then we just need to convert each clause into a CNF expression with 3 literals per clause.
    
    Suppose we have a clause with 1 literal: $a$.
    Convert this to $(a \lor u_1 \lor u_2) \land (a \lor u_1 \lor \neg u_2) \land (a \lor \neg u_1 \lor u_2) \land (a \lor \neg u_1 \lor \neg u_2)$.
    Suppose we have a clause with 2 literals: $a \lor b$.
    Convert this to $(a \lor b \lor u_1) \land (a \lor b \lor \neg u_1))$.
    
    Now suppose we have a clause with $n$ literals: $a \lor b \lor c \lor \ldots$.
    Convert this to $(a \lor b \lor u_1) \land (c \lor \neg u_1 \lor u_2)) \land \ldots \land (i \lor \neg u_{n-4} \lor u_{n-3}) \land (j \lor k \lor \neg u_{n-3})$.
  \end{alertblock}

\end{frame}